Mt/sample.lean
@@ -68,7 +68,7 @@ def thread1 : TaskM spec Unit :=do
 
 theorem thread1_valid : thread1.valid_for_reservation' ReservationInstance.empty :=by
   rw [valid_for_reservation']
-  apply valid_for_reservation_bind _ _ _ λ (r : spec.Reservation) _ => r.luft = 1
+  apply valid_for_reservation_bind _ _ _ (λ _ => true) λ (r : spec.Reservation) _ => r.luft = 1
   . -- validate ++x
     ---------------
     apply valid_for_reservation_rm
@@ -89,7 +89,7 @@ theorem thread1_valid : thread1.valid_for_reservation' ReservationInstance.empty
         x ≤ x + 1 :=Nat.le_succ _
   
   intro ⟨luft, min_x⟩ ⟨⟩ luft_def
-  apply valid_for_reservation_bind _ _ _ λ _ _ => True
+  apply valid_for_reservation_bind _ _ _ (λ _ => true) λ _ _ => True
   . -- validate ++y knowing luft = 1
     --------------------------------
     have luft_def : luft = 1 :=luft_def
@@ -107,11 +107,11 @@ theorem thread1_valid : thread1.valid_for_reservation' ReservationInstance.empty
   
   clear luft min_x luft_def
   intro ⟨luft, min_x⟩ ⟨⟩ ⟨⟩
-  apply valid_for_reservation_bind (spec :=spec) _ _ _ λ ⟨_, min_x⟩ y => min_x = y
+  apply valid_for_reservation_bind (spec :=spec) _ _ _ (λ _ => true) λ ⟨_, min_x⟩ y => min_x = y
   . -- validate `let py = y` with `min_x := py`
     -------------------------------------------
     apply valid_for_reservation_read
-    intro ⟨x, y⟩ ⟨env_luft, (env_min_x : Nat)⟩ initial_valid
+    intro ⟨x, y⟩ ⟨env_luft, (env_min_x : Nat)⟩ initial_valid _
     simp only [and_true]
 
     have : x ≥ y + (env_luft + luft) ∧ x ≥ Nat.max env_min_x min_x :=initial_valid
@@ -134,12 +134,12 @@ theorem thread1_valid : thread1.valid_for_reservation' ReservationInstance.empty
 
   clear luft min_x
   intro ⟨luft, min_x⟩ (py : Nat) min_x_def
-  apply valid_for_reservation_bind (spec :=spec) _ _ _ λ _ x => x ≥ py
+  apply valid_for_reservation_bind (spec :=spec) _ _ _ (λ _ => true) λ _ x => x ≥ py
   . -- validate `let px = x` knowing min_x = py
     -------------------------------------------
     have min_x_def : min_x = py :=min_x_def
     apply valid_for_reservation_read
-    intro ⟨x, y⟩ ⟨env_luft, (env_min_x : Nat)⟩ initial_valid
+    intro ⟨x, y⟩ ⟨env_luft, (env_min_x : Nat)⟩ initial_valid _
 
     have : x ≥ y + (env_luft + luft) ∧ x ≥ Nat.max env_min_x min_x :=initial_valid
     show (x ≥ y + env_luft ∧ x ≥ Nat.max env_min_x 0) ∧ x ≥ py
